driver/CallConv.v
@@ -49,518 +49,23 @@ Unset Program Cases.
 Coercion cc_c : cklr >-> callconv.
 
 
-(** * Stacking *)
-
-(** The simulation conventions for most passes are simple enough that
-  we can express them directly as [R @ CC], where [R] is a CKLR
-  matching the memory relation used in the simulation proof, and
-  [CC] expresses the structural correspondance between source- and
-  target-level queries and replies. However, the Stacking pass
-  involves fairly complex invariants and it is simpler to formulate
-  the corresponding simulation convention as a monolithic one, closely
-  coupled with the corresponding simulation proof.
-
-  In the following we show that this simulation convention can then be
-  decoupled into a CKLR and a structural convention. This form is then
-  used as the outside interface for the pass and integrated to the
-  strategy outlined above. *)
-
-Require Import Classical.
-
-(** ** Structural convention *)
-
-(** The first step is to define the structural convention we will be
-  using between [li_locset] and [li_mach]. *)
-
-(** *** Dealing with the arguments region *)
-
-(* One key aspect of this convention is the encoding of arguments: at
-  the source level, arguments for the call are stored in abstract
-  locations, which become either registers or in-memory stack slots at
-  the target level. Crucially, these stack slots must not be
-  accessible as memory locations in the source program, otherwise the
-  invariant relating abstract and concrete stack locations may be
-  broken through aliasing. Hence, in the structural convention the
-  source memory cannot be *equal* to the target memory, but instead
-  must be a version of the target memory where permissions on the
-  arguments region of the stack haven been removed.
-
-  This can be obtained using the memory operation [Mem.free]. However,
-  for some of the properties we need the corresponding memory state
-  cannot be freely chosen, and we must instead use the following
-  characterization. *)
-
-Definition loc_outside_range (b: block) (lo hi: Z) :=
-  fun b' ofs => b = b' -> ~ lo <= ofs < hi.
-
-Record free_spec m b lo hi m_ :=
-  {
-    free_spec_range_perm: Mem.range_perm m b lo hi Cur Freeable;
-    free_spec_no_perm ofs k p: lo <= ofs < hi -> ~ Mem.perm m_ b ofs k p;
-    free_spec_unchanged: Mem.unchanged_on (loc_outside_range b lo hi) m m_;
-    free_spec_nextblock: Mem.nextblock m_ = Mem.nextblock m;
-  }.
-
-Lemma free_free_spec m b lo hi m':
-  Mem.free m b lo hi = Some m' ->
-  free_spec m b lo hi m'.
-Proof.
-  split.
-  - eapply Mem.free_range_perm; eauto.
-  - eapply Mem.perm_free_2; eauto.
-  - eapply Mem.free_unchanged_on; eauto.
-    unfold loc_outside_range. clear. firstorder.
-  - eapply Mem.nextblock_free; eauto.
-Qed.
-
-Lemma free_spec_perm_outside_range m b lo hi m_ b' ofs k p:
-  free_spec m b lo hi m_ ->
-  Mem.perm m_ b' ofs k p ->
-  loc_outside_range b lo hi b' ofs.
-Proof.
-  intros Hm_ Hp Hb' Hofs. subst.
-  eapply free_spec_no_perm; eauto.
-Qed.
-
-Lemma free_spec_valid_block m b lo hi m_ b':
-  free_spec m b lo hi m_ ->
-  Mem.valid_block m b' <-> Mem.valid_block m_ b'.
-Proof.
-  intro. unfold Mem.valid_block. erewrite <- free_spec_nextblock; eauto. tauto.
-Qed.
-
-Lemma free_spec_perm m b lo hi m_ b' ofs k p:
-  free_spec m b lo hi m_ ->
-  loc_outside_range b lo hi b' ofs ->
-  Mem.perm m b' ofs k p <-> Mem.perm m_ b' ofs k p.
-Proof.
-  intros; split; intro Hp;
-  eapply (Mem.unchanged_on_perm _ m m_); eauto using free_spec_unchanged;
-  eapply Mem.perm_valid_block in Hp; eauto.
-  rewrite free_spec_valid_block; eauto.
-Qed.
-
-Lemma free_spec_perm_3 m b lo hi m_ b' ofs k p:
-  free_spec m b lo hi m_ ->
-  Mem.perm m_ b' ofs k p ->
-  Mem.perm m b' ofs k p.
-Proof.
-  intros. rewrite free_spec_perm; eauto using free_spec_perm_outside_range.
-Qed.
-
-Lemma free_spec_extends m b lo hi m_:
-  free_spec m b lo hi m_ ->
-  Mem.extends m_ m.
-Proof.
-  intros Hm_.
-  split.
-  - eapply free_spec_nextblock; eauto.
-  - split; inversion 1; clear H; subst; rewrite ?Z.add_0_r.
-    + intros Hp. eapply free_spec_perm; eauto using free_spec_perm_outside_range.
-    + intros _. apply Z.divide_0_r.
-    + intros Hp. erewrite (Mem.unchanged_on_contents _ m m_).
-      * destruct ZMap.get; constructor. apply val_inject_refl.
-      * eapply free_spec_unchanged; eauto.
-      * eapply free_spec_perm_outside_range; eauto.
-      * eapply free_spec_perm_3; eauto.
-  - intros b' ofs k p Hp.
-    destruct (classic (loc_outside_range b lo hi b' ofs)).
-    + erewrite <- free_spec_perm; eauto.
-    + right. unfold loc_outside_range in H.
-      assert (b = b' /\ lo <= ofs < hi) as [Hb Hofs] by tauto. subst b'. clear H.
-      eapply free_spec_no_perm; eauto.
-Qed.
-
-Lemma free_spec_inject_inv f m1 m2 b lo hi m2_:
-  free_spec m2 b lo hi m2_ ->
-  Mem.inject f m1 m2 ->
-  (forall ofs, lo <= ofs < hi -> loc_out_of_reach f m1 b ofs) ->
-  Mem.inject f m1 m2_.
-Proof.
-  intros Hm2_ Hm Hp. destruct Hm. split; auto.
-  - destruct mi_inj. split; auto.
-    + intros b1 b2 delta ofs k p Hb Hp'. erewrite <- free_spec_perm; eauto.
-      intros Hb2 Hofs. destruct Hb2. eapply Hp; eauto.
-      replace (ofs + delta - delta) with ofs by xomega.
-      eauto 3 with mem.
-    + intros b1 ofs b2 delta Hb Hp'.
-      erewrite (Mem.unchanged_on_contents _ m2 m2_); eauto.
-      * eapply free_spec_unchanged; eauto using free_spec_perm_outside_range.
-      * eapply free_spec_perm_outside_range; eauto.
-        erewrite <- free_spec_perm; eauto.
-        intros Hb2 Hofs. subst. eapply Hp; eauto.
-        replace (ofs + delta - delta) with ofs by xomega.
-        eauto with mem.
-  - intros. erewrite <- free_spec_valid_block; eauto.
-  - eauto using free_spec_perm_3.
-Qed.
-
-Lemma free_spec_unfree m b lo hi m_:
-  Mem.range_perm m b lo hi Cur Freeable ->
-  (forall ofs k p, lo <= ofs < hi -> ~ Mem.perm m_ b ofs k p) ->
-  Pos.le (Mem.nextblock m) (Mem.nextblock m_) ->
-  exists m',
-    free_spec m' b lo hi m_ /\
-    Mem.unchanged_on (fun b' ofs => b = b' /\ lo <= ofs < hi) m m'.
-Proof.
-  (* mix m and m_ to recover the region from m in m' *)
-Admitted.
-
-Lemma free_spec_inject f m1 m2 b1 b2 delta lo hi m1_:
-  free_spec m1 b1 lo hi m1_ ->
-  Mem.inject f m1 m2 ->
-  f b1 = Some (b2, delta) ->
-  exists m2_,
-    Mem.free m2 b2 (lo + delta) (hi + delta) = Some m2_ /\
-    Mem.inject f m1_ m2_.
-Admitted.
-
-(** *** Definition *)
-
-(** We can now define the structural convention. *)
-
-Record cc_lm_world :=
-  lmw {
-    lmw_sg : signature;
-    lmw_ls : Locmap.t;
-    lmw_m : mem;
-    lmw_sb : block;
-    lmw_sofs : ptrofs;
-  }.
-
-Definition args_removed sg sb sofs m m_ :=
-  free_spec m sb (offset_sarg sofs 0) (offset_sarg sofs (size_arguments sg)) m_ /\
-  forall ofs, 0 <= ofs < size_arguments sg -> offset_fits sofs ofs.
-
-Definition args_stored sg ls m sb sofs :=
-  forall ofs ty,
-    let l := S Outgoing ofs ty in
-    In l (regs_of_rpairs (loc_arguments sg)) ->
-    Mem.load (chunk_of_type ty) m sb (offset_sarg sofs ofs) = Some (ls l).
-(* /\
-    offset_fits sofs ofs. *)
-
-Inductive cc_locset_mach_mq: cc_lm_world -> locset_query -> mach_query -> Prop :=
-  cc_locset_mach_mq_intro sg vf ls m_ rs sb sofs ra m:
-    (forall r, ls (R r) = rs r) ->
-    args_removed sg sb sofs m m_ ->
-    args_stored sg ls m sb sofs ->
-    Val.has_type ra Tptr ->
-    cc_locset_mach_mq
-      (lmw sg ls m sb sofs)
-      (lq vf sg ls m_)
-      (mq vf (Vptr sb sofs) ra rs m).
-
-Inductive cc_locset_mach_mr: cc_lm_world -> locset_reply -> mach_reply -> Prop :=
-  cc_locset_mach_mr_intro sg ls ls' m'_ sb sofs m rs' m':
-    (forall r, In r (regs_of_rpair (loc_result sg)) -> rs' r = ls' (R r)) ->
-    (forall r, is_callee_save r = true -> rs' r = (ls (R r))) ->
-    args_removed sg sb sofs m' m'_ ->
-    Mem.unchanged_on (loc_init_args sb sofs (size_arguments sg)) m m' ->
-    cc_locset_mach_mr (lmw sg ls m sb sofs) (lr ls' m'_) (mr rs' m').
-
-Program Definition cc_locset_mach: callconv li_locset li_mach :=
-  {|
-    match_senv _ := eq;
-    match_query := cc_locset_mach_mq;
-    match_reply := cc_locset_mach_mr;
-  |}.
-
-(** ** Mixing memory states *)
-
-(** For incoming calls, [Stacking] uses the simulation convention
-  [cc_locset inj @ cc_locset_mach]. However, the proof does not keep
-  track of an intermediate memory state. This means that to prove that
-  replies are related, we first need to exhibit an intermediate memory
-  state such that 1. freeing the arguments region yields the
-  source-level memory, and 2. this arguments region is unchanged with
-  respect the corresponding memory state of the query.
-
-  To achieve this we use the following construction:
-  [Mem_mix m' b lo hi m] merges the region of [m] specified by
-  [(b, lo, hi)] into [m']. The intention is that if [m'] was obtained
-  from [m] by [Mem.free], potentially followed by additional
-  operations, [Mem_mix] will "undo" the free. *)
-
-Parameter Mem_mix : mem -> block -> Z -> Z -> mem -> option mem.
-
-Axiom Mem_mix_free_spec:
-  forall m' b lo hi m m'',
-    Mem_mix m' b lo hi m = Some m'' ->
-    free_spec m'' b lo hi m'.
-
-Axiom Mem_mix_unchanged:
-  forall m' b lo hi m m'',
-    Mem_mix m' b lo hi m = Some m'' ->
-    Mem.unchanged_on (fun b1 ofs1 => ~ (b = b1 /\ lo <= ofs1 < hi)) m' m''.
-
-Axiom Mem_mix_updated:
-  forall m' b lo hi m m'',
-    Mem_mix m' b lo hi m = Some m'' ->
-    Mem.unchanged_on (fun b1 ofs1 => b = b1 /\ lo <= ofs1 < hi) m m''.
-
-Axiom Mem_nextblock_mix:
-  forall m' b lo hi m m'',
-    Mem_mix m' b lo hi m = Some m'' ->
-    Mem.nextblock m'' = Mem.nextblock m'.
-
-Axiom Mem_mix_extends:
-  forall m1' m2' b lo hi m1 m2 m2'',
-    Mem_mix m2' b lo hi m2 = Some m2'' ->
-    Mem.extends m1' m2' ->
-    Mem.extends m1 m2 ->
-    exists m1'',
-      Mem_mix m1' b lo hi m1 = Some m1'' /\
-      Mem.extends m1'' m2''.
-
-Axiom Mem_mix_inject:
-  forall f' m1' m2' b lo hi f m1 m2 m2'',
-    Mem_mix m2' b lo hi m2 = Some m2'' ->
-    Mem.inject f' m1' m2' ->
-    Mem.inject f m1 m2 ->
-    inject_incr f f' ->
-    exists m1'',
-      Mem_mix m1' b lo hi m1 = Some m1'' /\
-      Mem.inject f' m1'' m2''.
-
-Axiom Mem_mix_inject_left:
-  forall f f' m1 m2 m1' m2' b1 b2 delta lo hi m1'',
-    Mem_mix m1' b1 lo hi m1 = Some m1'' ->
-    Mem.inject f m1 m2 ->
-    Mem.inject f' m1' m2' ->
-    f b1 = Some (b2, delta) ->
-    Mem.unchanged_on (fun b ofs => b = b2 /\ lo + delta <= ofs < hi + delta) m2 m2' ->
-    Mem.inject f' m1'' m2'.
-
-(** ** Matching [cc_stacking] *)
-
-(** With this, we can prove the simulation convention refinements
-  property we need to match the Stacking proof. *)
-
-(** *** Incoming calls *)
-
-Lemma offset_sarg_inject f m1 m2 sb1 sb2 delta sofs1 sofs2 ofs sz:
-  Mem.inject f m1 m2 ->
-  Mem.range_perm m1 sb1 (offset_sarg sofs1 0) (offset_sarg sofs1 sz) Cur Freeable ->
-  (forall ofs, 0 <= ofs <= sz -> offset_fits sofs1 ofs) ->
-  0 <= ofs <= sz ->
-  f sb1 = Some (sb2, delta) ->
-  sofs2 = Ptrofs.add sofs1 (Ptrofs.repr delta) ->
-  offset_fits sofs2 ofs /\
-  offset_sarg sofs2 ofs = offset_sarg sofs1 ofs + delta.
-Proof.
-  intros Hm Hp Hofs_sz FITS Hsb Hsofs.
-  erewrite ?(access_fits sofs1 _) in * by (apply Hofs_sz; xomega).
-  unfold offset_fits, offset_sarg in *.
-Abort.
-
-Lemma cc_lm_stacking:
-  ccref (cc_locset_mach @ cc_mach inj) (cc_stacking inj).
-Proof.
-  intros [[_ wlm] w] se1 se2 q1 q2 [[ ] Hse] (qi & Hq1i & Hqi2). cbn in *.
-  destruct Hqi2. inv Hq1i.
-  inversion H2 as [ | | | | ? ? sb2 sofs2 sdelta Hsb Hsofs | ]; clear H2; subst.
-  exists (stkw inj w sg ls sb2 (Ptrofs.add sofs (Ptrofs.repr sdelta)) m2).
-  split; [ | split].
-  - cbn. auto.
-  - destruct H15 as [FREE FITS].
-    constructor; auto.
-    + setoid_rewrite H13. auto.
-    + cbn. repeat apply conj.
-      * admit.
-      * apply Mem.unchanged_on_refl.
-      * admit.
-      * intros ofs ty REG.
-        admit.
-    + assert (Mem.extends m_ m1) by eauto using free_spec_extends.
-      destruct H6; cbn in *. erewrite <- Mem.mext_next by eauto. constructor.
-      eapply Mem.extends_inject_compose; eauto.
-    + admit.
-    + destruct H4; cbn in *; congruence.
-  - intros r1 r2 Hr. inv Hr.
-    assert
-      (exists m1'',
-          Mem_mix m1' sb (offset_sarg sofs 0) (offset_sarg sofs (size_arguments sg)) m1 = Some m1'')
-      as [m1'' Hm1''] by admit.
-    eassert _ by (eapply Mem_mix_free_spec; eauto).
-    set (rs1' r := if is_callee_save r then ls (R r) else
-                   if in_dec mreg_eq r (regs_of_rpair (loc_result sg)) then ls1' (R r) else
-                   Vundef).
-    exists (mr rs1' m1''). split.
-    + constructor.
-      * subst rs1'. intros r REG. cbn.
-        destruct in_dec; try contradiction.
-        replace (is_callee_save r) with false; auto.
-        pose proof (loc_result_caller_save sg) as Hr.
-        destruct loc_result; cbn in *; intuition congruence.
-      * subst rs1'. intros r REG. cbn.
-        rewrite REG. congruence.
-      * destruct H15. split; auto.
-      * eapply Mem.unchanged_on_implies.
-        -- eapply Mem_mix_updated; eauto.
-        -- destruct 1; eauto.
-    + exists w'; split; auto.
-      constructor.
-      * intros r. subst rs1'. cbn.
-        destruct is_callee_save eqn:CSR; eauto.
-        destruct in_dec; eauto.
-      * destruct H6. inv H18. inv H21. cbn in *.
-        erewrite <- Mem_nextblock_mix by eauto. constructor.
-        eapply Mem_mix_inject_left; eauto.
-        eapply Mem.unchanged_on_implies; eauto.
-        intros b ofs [Hb Hofs] VLD. subst. constructor.
-        admit. (* ptr arith *)
-Admitted.
-
-(** *** Outgoing calls *)
-
-(** The following construction is needed both for the commutation
-  property associated with [cc_locset_mach] and [cc_mach] and in the
-  simulation proof for external calls in [Stacking]. It is used to
-  formulate an [li_locset] view of an [li_mach] query. *)
-
-Definition make_locset (rs: Mach.regset) (m: mem) (sp: val) (l: loc) : val :=
-  match l with
-    | R r => rs r
-    | S Outgoing ofs ty =>
-      let v := load_stack m sp ty (Ptrofs.repr (fe_ofs_arg + 4 * ofs)) in
-      Val.maketotal v
-    | _ => Vundef
-  end.
-
-Lemma cc_stacking_lm:
-  ccref (cc_stacking injp) (cc_locset injp @ cc_locset_mach).
-Proof.
-  intros w se1 se2 q1 q2 Hse Hq. destruct Hq. cbn in * |- .
-  destruct H2 as (? & ? & ? & ?).
-  set (ls2 := make_locset rs2 m2 (Vptr sb2 sofs2)).
-  edestruct (Mem.range_perm_free m2) as (m2_ & Hm2_); eauto.
-  destruct H3; inv Hse; cbn in * |- .
-  eassert (Hm_ : _). {
-    eapply Mem.free_right_inject; eauto.
-    intros. eapply H4; eauto.
-    + constructor; eauto.
-    + replace (ofs + delta - delta) with ofs by xomega.
-    eapply Mem.perm_max, Mem.perm_implies; eauto. constructor.
-  }
-  exists (se2, (sg, injpw _ _ _ Hm_), lmw sg ls2 m2 sb2 sofs2). repeat apply conj.
-  - constructor; cbn; auto. constructor; auto. 
-    erewrite Mem.nextblock_free; eauto.
-  - exists (lq vf2 sg ls2 m2_). split.
-    + constructor; eauto.
-      * intros r Hr. destruct Hr; cbn -[Z.add Z.mul]; eauto.
-        edestruct H8 as (v2 & Hv2 & Hv); eauto.
-        admit. (* ptr arith *)
-      * constructor.
-    + econstructor; eauto.
-      * split; eauto using free_free_spec.
-      * intros ofs ty l REG. subst l ls2. cbn -[Z.add Z.mul].
-        edestruct H8 as (v2 & Hv2 & Hv); eauto.
-        rewrite Hv2. admit. (* ptr arith *)
-  - intros r1 r2 (ri & (w' & Hw' & Hr1i) & Hri2). cbn in *.
-    inv Hw'. inv Hr1i. inv H9. inv Hri2. destruct H28. cbn in *.
-    rename m1'0 into m1'. rename m2'0 into m2'_. rename m' into m2'. 
-    assert (Hm'' : Mem.inject f' m1' m2'). {
-      eapply Mem.inject_extends_compose; eauto.
-      eapply free_spec_extends; eauto.
-    }
-    exists (injpw f' m1' m2' Hm''); cbn.
-    + constructor; eauto.
-      * intros b ofs p Hb Hp.
-        admit. (* permission inversion on free_spec etc. *)
-      * admit. (* the unchanged_on mixing *)
-      * red. unfold Mem.valid_block. erewrite <- (Mem.nextblock_free m2); eauto.
-    + intros r REG. rewrite H26; eauto.
-    + intros r REG. rewrite H27; eauto.
-    + constructor.
-    + auto.
-Admitted.
-
-(** *** Typing of [cc_locset_mach] source state *)
-
-(** This only works for [Archi.ptr64 = true], in which case there are
-  no actual constraints on register typing. But we need to rely on
-  this for now because of the way callee-save register preservation is
-  formulated in the stacking proof: there is only a guarantee that the
-  original query's source-level register still inject into the reply's
-  target-level registers, but there is no guarantee that the
-  target-level registers are actually unchanged. This means that on
-  incoming calls, [cc_locset_mach] must occur first, before the [inj]
-  component, if we are to satisfy the associated preservation property.
-  But this means that the [lessdef_loc] component which we must insert
-  after [wt_loc] for commutation purposes cannot be absorbed into
-  [inj], and for similar reasons it cannot be folded into
-  [cc_stacking] either.
-
-  So we work around it using the following properties. *)
-
-Lemma type_of_chunk_of_type ty:
-  type_of_chunk (chunk_of_type ty) = ty.
-Proof.
-  destruct ty; cbn; auto.
-Qed.
-
-Lemma always_has_mreg_type v r:
-  Val.has_type v (mreg_type r).
-Proof.
-  unfold mreg_type. change Archi.ptr64 with true.
-  destruct v, r; cbn; auto.
-Qed.
-
-Lemma wt_loc_out_of_thin_air:
-  cceqv (wt_loc @ cc_locset_mach) cc_locset_mach.
-Proof.
-  split.
-  - intros [[xse [xxse sg]] w] se1 se2 q1 q2 [[Hsei] Hse] (_ & [Hq1] & Hq).
-    inv Hsei. inv Hq1. exists w; repeat apply conj; auto.
-    intros r1 r2 Hr. destruct Hr; cbn in *.
-    eexists. split; constructor; auto. constructor.
-    intros r Hr. apply always_has_mreg_type.
-  - intros w se _ q1 q2 [ ] Hq. destruct Hq.
-    exists (se, (se, sg), lmw sg ls m sb sofs). cbn. repeat apply conj; auto.
-    + constructor. auto.
-    + eexists. split; constructor; auto. constructor.
-      intros l Hl. destruct Hl.
-      * apply always_has_mreg_type.
-      * cbn. rewrite <- (type_of_chunk_of_type ty) at 2.
-        eapply Mem.load_type. eauto.
-    + intros r1 r2 (_ & [Hr1] & Hr). auto.
-Qed.
-
-Instance wt_loc_qprop R:
-  PropagatesQueryInvariant (cc_locset R) wt_loc.
-Proof.
-  constructor. cbn.
-  intros [sg wR] [? xsg] se1 se2 q1 q2 Hse Hxse Hq Hq2. subst. inv Hq. inv Hq2.
-  exists (se1, sg). split; auto. constructor.
-  intros. eapply val_has_type_inject; eauto. red. eauto.
-Qed.
-
-Instance wt_loc_rprop R:
-  PropagatesReplyInvariant (cc_locset R) wt_loc.
-Proof.
-  constructor. cbn.
-  intros [se ?] [sg wR] [? ?] se1 se2 q1 q2 r1 r2 Hse ? ? Hq Hq1 Hq2 (wR' & HwR' & Hr) Hr2.
-  subst. inv Hq. inv Hq1. inv Hq2. inv Hr. inv Hr2. constructor.
-  intros. eapply val_has_type_inject; eauto. red. eauto.
-Qed.
-
-
-(** * Commutable typing constraints *)
-
-(** The typing invariants [wt_c] and [wt_loc] do not commute with
-  CKLRs, however the following alternative formulations of the typing
-  constraints do. The idea is that source values are forced to
-  [Vundef] when the target values are ill-typed. The gap can then be
-  absorbed into a CKLR to recover the original invariant. *)
-
-
 (** * Commutation properties *)
+
+(** First, we define a general form for the commutation properties we
+  need, and prove the straightforward ones. *)
 
 (** ** Basic setup *)
 
+(** The following class captures a general commutation property.
+  In general, [cc] will be a structural simulation convention;
+  [R1] and [R2] will be corresponding source- and target-level CKLR
+  simulation conventions. *)
+
 Class Commutes {liA liB} (cc: callconv liA liB) R1 R2 :=
   commute : ccref (cc @ R2) (R1 @ cc).
+
+(** The following lemma provides a convenient way to use [commute] for
+  rewriting within more complex sequences of simulation conventions. *)
 
 Lemma commute_around `{Commutes} {liC} (x : callconv liB liC):
   ccref (cc @ R2 @ x) (R1 @ cc @ x).
@@ -570,6 +75,8 @@ Proof.
 Qed.
 
 Arguments commute_around {liA liB} cc {R1 R2 H liC x}.
+
+(** Finally, we provide some composite instances for [Commutes]. *)
 
 Instance commut_join {liA liB} cc R1 R2 S1 S2 :
   @Commutes liA liB cc R1 R2 ->
@@ -605,8 +112,9 @@ Qed.
 (** ** [cc_c_locset] *)
 
 (** The commutation of [cc_c_locset] basically follows the way the
-  original LTL semantics evaluates calls to external functions: we
-  read out the arguments from the location set, then write back the
+  original LTL semantics evaluates calls to external functions:
+  for queries, we read out the arguments from the location set;
+  once we get a C reply, we write back the
   result and mark the appropriate registers undefined. *)
 
 Lemma locmap_getpair_inject f ls1 ls2 p:
@@ -652,114 +160,9 @@ Proof.
       * admit. (* loc pairs *)
 Admitted.
 
-(** ** [cc_locset_mach] *)
-
-(** For queries, we need to synthesizing the target-level locset by
-  extracting arguments from the memory and then removing them. *)
-
-(*
-Lemma match_agree_args R w sg m1 m2 sp1 sp2 ls1 rs2:
-  agree_args sg m1 sp1 ls1 ->
-  match_mem R w m1 m2 ->
-  Val.inject (mi R w) sp1 sp2 ->
-  (forall r, Val.inject (mi R w) (ls1 (Locations.R r)) (rs2 r)) ->
-  exists ls2,
-    agree_args sg m2 sp2 ls2 /\
-    (forall r, ls2 (Locations.R r) = rs2 r) /\
-    loc_external_rel sg (Val.inject (mi R w)) ls1 ls2.
-Proof.
-  intros Hargs1 Hm Hsp Hrs.
-  exists (make_locset rs2 m2 sp2).
-  repeat apply conj.
-  - intros ofs ty l Hl. subst l. specialize (Hargs1 ofs ty Hl). clear - Hargs1 Hm Hsp.
-    unfold load_stack in Hargs1. transport Hargs1.
-    cbn [make_locset]. setoid_rewrite H. reflexivity.
-  - auto.
-  - intros l Hl. destruct Hl.
-    + cbn. auto.
-    + specialize (Hargs1 ofs ty H). clear - Hargs1 Hm Hsp.
-      unfold load_stack in Hargs1. transport Hargs1.
-      cbn [make_locset]. setoid_rewrite H. cbn. auto.
-Qed.
-
-Instance cklr_free_args R:
-  Monotonic free_args
-    (|= - ==> match_mem R ++> Val.inject @@ [mi R] ++> k1 option_le (<> match_mem R)).
-Proof.
-  intros w sg m1 m2 Hm sp1 sp2 Hsp.
-  destruct (free_args sg m1 sp1) as [m1_ | ] eqn:H1; [ | constructor].
-  unfold free_args in H1. destruct sp1 as [ | | | | | sb1 sofs1]; try discriminate.
-  cut (exists w' m2_, w ~> w' /\ free_args sg m2 sp2 = Some m2_ /\ match_mem R w' m1_ m2_).
-  - intros (? & ? & ? & ? & ?). rewrite H0. rauto.
-  - revert m1 m2 Hm m1_ H1. inv Hsp. revert w H1. cbn [free_args].
-    induction regs_of_rpairs.
-    + cbn. intros. inv H0. exists w, m2. split; auto. reflexivity.
-    + destruct a as [ | [ ]]; cbn -[Z.add Z.mul acc] in *; auto.
-      intros. destruct Mem.free eqn:Hm1_ in H0; try discriminate.
-      eapply transport in Hm1_. 2: {
-        clear Hm1_. repeat rstep.
-        eapply ptrbits_ptr_inject; eauto.
-        eapply H. pose proof (size_chunk_pos (chunk_of_type ty)). xomega.
-      }
-      destruct Hm1_ as (m2_ & Hm2_ & w' & Hw' & Hm_).
-      edestruct (IHl w') as (w'' & m2__ & Hw'' & Hm2__ & Hm__); eauto.
-      { eapply mi_acc; eauto. }
-      exists w'', m2__. split; [rauto | ].
-      rewrite <- Ptrofs.add_assoc, Hm2_.
-      eauto.
-Qed.
-*)
-
-Instance bis f b1 b2:
-  RExists (f b1 = Some (b2, 0)) (block_inject_sameofs f) b1 b2.
-Proof.
-  firstorder.
-Qed.
-
-Instance loc_external_subrel:
-  Monotonic loc_external_rel (- ==> subrel ++> subrel).
-Proof.
-  unfold loc_external_rel. repeat rstep.
-  red. intros. auto.
-Qed.
-
-Instance commut_locset_mach R:
-  Commutes cc_locset_mach (cc_locset R) (cc_mach R).
-Proof.
-Admitted.
-(*
-  intros [[_ [sg ls1]] wR] se1 se2 q1 q2 [[ ] Hse2] (qi & Hq1i & Hqi2).
-  cbn in * |- . destruct Hqi2. inv Hq1i. rename m' into m1_. rename ls into ls1.
-
-  (** Synthesizing the query *)
-  transport H14. rename x into m2_.
-  edestruct match_agree_args as (ls2 & Hargs2 & Hrs2 & Hls); eauto.
-  { intro r. rewrite H15. eauto. }
-  set (ls2wt l := Val.ensure_type (ls2 l) (Loc.type l)).
-
-  exists (se2, (sg, wR'), (sg, rs2)). repeat apply conj.
-  - cbn. split; rauto.
-  - exists (lq vf2 sg ls2 m2_). split.
-    + econstructor; try rauto; auto.
-    + constructor; eauto.
-      destruct H4; cbn in *; congruence.
-  - intros r1 r2 (ri & (wR'' & HwR'' & Hr1i) & Hri2). 
-    destruct Hr1i. inv Hri2. rename rs' into rs2'.
-    set (rs1' r := result_regs sg ls1 ls1' (Locations.R r)).
-    exists (mr rs1' m1'). split.
-    + constructor; auto.
-      * intros r Hr. unfold rs1'. rewrite <- result_regs_agree_callee_save; auto.
-      * intros r Hr. unfold rs1'. cbn. destruct in_dec; tauto.
-    + exists wR''. split; [rauto | ]. constructor; auto.
-      intro r. unfold rs1', result_regs.
-      destruct in_dec. { rewrite H18; auto. }
-      destruct is_callee_save eqn:Hr; auto.
-      rewrite H14 by auto. rewrite H15. generalize (H5 r).
-      repeat rstep. change (wR ~> wR''). rauto.
-Qed.
-*)
-
 (** ** [cc_mach_asm] *)
+
+(** The commutation property for [cc_mach_asm] is straightforward. *)
 
 Instance commut_mach_asm R:
   Commutes cc_mach_asm (cc_mach R) (cc_asm R).
@@ -786,7 +189,7 @@ Admitted.
 
 (** * Typing invariants *)
 
-(** On their own, the typing invariants [wt_c] and [wt_locset] do not
+(** On their own, the typing invariants [wt_c] and [wt_loc] do not
   commute with CKLRs. This is because a source value may be [Vundef],
   hence well-typed, even when the target value is defined but ill-typed.
   However, we can recover a sufficient commutation property by
@@ -987,3 +390,548 @@ Proof.
     + apply (inv_drop _ _).
   - repeat rstep. apply cc_join_ub_l.
 Qed.
+
+
+(** * Stacking *)
+
+(** The simulation conventions for most passes are simple enough that
+  we can express them directly as [R @ CC], where [R] is a CKLR
+  matching the memory relation used in the simulation proof, and
+  [CC] expresses the structural correspondance between source- and
+  target-level queries and replies. However, the Stacking pass
+  involves fairly complex invariants and it is simpler to formulate
+  the corresponding simulation convention as a monolithic one, closely
+  coupled with the corresponding simulation proof.
+
+  In the following we show that this simulation convention can then be
+  decoupled into a CKLR and a structural convention. This form is then
+  used as the outside interface for the pass and integrated to the
+  strategy outlined above. *)
+
+Require Import Classical.
+
+(** ** Structural convention *)
+
+(** The first step is to define the structural convention we will be
+  using between [li_locset] and [li_mach]. *)
+
+(** *** Dealing with the arguments region *)
+
+(** One key aspect of this convention is the encoding of arguments: at
+  the source level, arguments for the call are stored in abstract
+  locations, which become either registers or in-memory stack slots at
+  the target level. Crucially, these stack slots must not be
+  accessible as memory locations in the source program, otherwise the
+  invariant relating abstract and concrete stack locations may be
+  broken through aliasing. Hence, in the structural convention the
+  source memory cannot be *equal* to the target memory, but instead
+  must be a version of the target memory where permissions on the
+  arguments region of the stack have been removed.
+
+  For queries, this can be expressed using [Mem.free]. We also deal
+  separately with the case where no arguments are stored in the stack.
+  This is both to ensure the compatibility of [args_removed] with
+  injection, and to allow [Vnullptr] as a possible stack pointer for
+  the initial call to [main()]. *)
+
+Inductive args_removed sg: val -> mem -> mem -> Prop :=
+  | args_removed_tailcall_possible sp m:
+      tailcall_possible sg ->
+      args_removed sg sp m m
+  | args_removed_free sb sofs m m_:
+      Mem.free m sb (offset_sarg sofs 0) (offset_sarg sofs (size_arguments sg)) = Some m_ ->
+      (forall ofs, 0 <= ofs < size_arguments sg -> offset_fits sofs ofs) ->
+      size_arguments sg > 0 ->
+      (forall ofs ty,
+        In (S Outgoing ofs ty) (regs_of_rpairs (loc_arguments sg)) ->
+        exists v, load_stack m (Vptr sb sofs) ty (Ptrofs.repr (fe_ofs_arg + 4 * ofs)) = Some v) ->
+      args_removed sg (Vptr sb sofs) m m_.
+
+(** This takes care of how the LTL memory state is obtained from the
+  Mach-level one. In addition, the following construction reconstructs
+  the LTL-level [locset] from the Mach-level [regset] by reading the
+  additional stack locations from the Mach memory. *)
+
+Definition make_locset (rs: Mach.regset) (m: mem) (sp: val) (l: loc) : val :=
+  match l with
+    | R r => rs r
+    | S Outgoing ofs ty =>
+      let v := load_stack m sp ty (Ptrofs.repr (fe_ofs_arg + 4 * ofs)) in
+      Val.maketotal v
+    | _ => Vundef
+  end.
+
+(** For replies, in some simulation convention refinement properties
+  we want to establish, the source memory state is often given to us
+  and we have to establish the relationship. This means we can't use
+  [Mem.free] in the same way; fortunately, it is enough to give a more
+  extensional characterization in terms of [Mem.unchanged] involving
+  the following address predicate. *)
+
+Definition not_init_args (sz: Z) (sp: val) :=
+  fun b ofs => ~ loc_init_args sz sp b ofs.
+
+(** *** Definition *)
+
+(** We can now define the structural convention
+  from [li_locset] to [li_mach]. *)
+
+Record cc_lm_world :=
+  lmw {
+    lmw_sg : signature;
+    lmw_rs : Mach.regset;
+    lmw_m : mem;
+    lmw_sp : val;
+  }.
+
+Inductive cc_locset_mach_mq: cc_lm_world -> locset_query -> mach_query -> Prop :=
+  cc_locset_mach_mq_intro sg vf m_ rs sp ra m:
+    args_removed sg sp m m_ ->
+    Val.has_type ra Tptr ->
+    cc_locset_mach_mq
+      (lmw sg rs m sp)
+      (lq vf sg (make_locset rs m sp) m_)
+      (mq vf sp ra rs m).
+
+Inductive cc_locset_mach_mr: cc_lm_world -> locset_reply -> mach_reply -> Prop :=
+  cc_locset_mach_mr_intro sg rs ls' m'_ sp m rs' m':
+    (forall r, In r (regs_of_rpair (loc_result sg)) -> rs' r = ls' (R r)) ->
+    (forall r, is_callee_save r = true -> rs' r = rs r) ->
+    Mem.unchanged_on (not_init_args (size_arguments sg) sp) m'_ m' ->
+    Mem.unchanged_on (loc_init_args (size_arguments sg) sp) m m' ->
+    cc_locset_mach_mr (lmw sg rs m sp) (lr ls' m'_) (mr rs' m').
+
+Program Definition cc_locset_mach: callconv li_locset li_mach :=
+  {|
+    match_senv _ := eq;
+    match_query := cc_locset_mach_mq;
+    match_reply := cc_locset_mach_mr;
+  |}.
+
+(** ** Commutation property *)
+
+(** For queries, we need to synthesizing the target-level locset by
+  extracting arguments from the memory and then removing them. *)
+
+Lemma offset_sarg_inject R w m1 m2 sb1 sofs1 sb2 sofs2 ofs:
+  match_mem R w m1 m2 ->
+  Mem.perm m1 sb1 (offset_sarg sofs1 0) Cur Freeable ->
+  ptrbits_inject (mi R w) (sb1, sofs1) (sb2, sofs2) ->
+  ptr_inject (mi R w) (sb1, offset_sarg sofs1 ofs) (sb2, offset_sarg sofs2 ofs).
+Proof.
+  intros Hm Hp Hsp. inv Hsp.
+  unfold offset_sarg in *. rewrite Z.add_0_r in Hp.
+  apply ptr_inject_shift.
+  eapply ptrbits_ptr_inject; eauto.
+  rewrite Ptrofs.add_assoc, (Ptrofs.add_commut (Ptrofs.repr _)), <- Ptrofs.add_assoc.
+  constructor; auto.
+Qed.
+
+Lemma offset_sarg_expand ofs sofs:
+  offset_sarg sofs ofs = offset_sarg sofs 0 + 4 * ofs.
+Proof.
+  unfold offset_sarg. xomega.
+Qed.
+
+Lemma offset_sarg_ptrrange_inject R w m1 m2 sb1 sofs1 sb2 sofs2 ofs:
+  match_mem R w m1 m2 ->
+  Mem.perm m1 sb1 (offset_sarg sofs1 0) Cur Freeable ->
+  ptrbits_inject (mi R w) (sb1, sofs1) (sb2, sofs2) ->
+  ptrrange_inject (mi R w)
+    (sb1, offset_sarg sofs1 0, offset_sarg sofs1 ofs)
+    (sb2, offset_sarg sofs2 0, offset_sarg sofs2 ofs).
+Proof.
+  intros. rewrite !(offset_sarg_expand ofs).
+  rstep. eapply offset_sarg_inject; eauto.
+Qed.
+
+Lemma offset_fits_inject R w m1 m2 sb1 sb2 delta sofs1 sofs2 ofs sz:
+  match_mem R w m1 m2 ->
+  Mem.range_perm m1 sb1 (offset_sarg sofs1 0) (offset_sarg sofs1 sz) Cur Freeable ->
+  0 <= ofs < sz ->
+  mi R w sb1 = Some (sb2, delta) ->
+  sofs2 = Ptrofs.add sofs1 (Ptrofs.repr delta) ->
+  offset_fits sofs1 ofs ->
+  offset_fits sofs2 ofs.
+Proof.
+  intros Hm PERM Hofs Hsb Hsofs2 FITS.
+  unfold offset_fits, offset_sarg in *. subst sofs2.
+  rewrite !(Ptrofs.add_commut sofs1).
+  rewrite !(Ptrofs.add_assoc (Ptrofs.repr delta)).
+  rewrite !(Ptrofs.add_commut (Ptrofs.repr delta)).
+  erewrite cklr_address_inject; eauto.
+  rewrite <- (Z.add_assoc _ delta), (Z.add_comm delta), Z.add_assoc.
+  setoid_rewrite FITS.
+  erewrite <- cklr_address_inject; eauto.
+  * eapply PERM. xomega.
+  * eapply PERM. xomega.
+Qed.
+
+Instance load_stack_inject R:
+  Monotonic load_stack
+    (|= match_mem R ++> Val.inject @@ [mi R] ++> - ==> - ==>
+        k1 option_le (Val.inject @@ [mi R])).
+Proof.
+  unfold load_stack. rauto.
+Qed.
+
+Instance args_removed_cklr R:
+  Monotonic args_removed
+    (|= - ==> Val.inject @@ [mi R] ++> match_mem R ++> k1 set_le (<> match_mem R)).
+Proof.
+  intros w sg sp1 sp2 Hsp m1 m2 Hm m1_ Hm1_.
+  destruct Hm1_ as [sp m1 | sb1 sofs1 m1 m1_ FREE FITS].
+  - exists m2. split; [ | rauto].
+    constructor; auto.
+  - inversion Hsp. subst.
+    set (sofs2 := Ptrofs.add _ _).
+    assert (forall ofs,
+      ptr_inject (mi R w) (sb1, offset_sarg sofs1 ofs) (b2, offset_sarg sofs2 ofs)).
+    {
+      intro. eapply offset_sarg_inject; eauto.
+      + eapply Mem.free_range_perm; eauto. unfold offset_sarg. xomega.
+      + constructor; auto.
+    }
+    assert
+        (ptrrange_inject (mi R w)
+                        (sb1, offset_sarg sofs1 0, offset_sarg sofs1 (size_arguments sg))
+                        (b2, offset_sarg sofs2 0, offset_sarg sofs2 (size_arguments sg))).
+    {
+      eapply ptr_ptrrange_inject; split; eauto.
+      unfold offset_sarg. xomega.
+    }
+    generalize FREE. transport FREE. intros FREE.
+    eexists; split.
+    + eapply args_removed_free; eauto.
+      * clear - Hm FITS H3 FREE.
+        intros ofs Hofs. eapply offset_fits_inject; eauto.
+        -- eapply Mem.free_range_perm; eauto.
+        -- reflexivity.
+      * intros ofs ty REG. edestruct H0 as [v Hv]; eauto.
+        transport Hv. eauto.
+    + rauto.
+Qed.
+
+Hint Extern 1 (Transport _ _ _ _ _) =>
+  set_le_transport @args_removed : typeclass_instances.
+
+(** For replies, the challenge is to construct a version of the source
+  memory state which contains the original arguments, and a version of
+  the source [Mach.regset] which contains the right mixture of
+  original callee-save registers and results from the reply's
+  locset. The following lemmas will help. *)
+
+Lemma result_mem R sz sp1 sp2 w m1 m2 w' m1'_ m2'_ m2':
+  w ~> w' ->
+  Val.inject (mi R w) sp1 sp2 ->
+  match_mem R w m1 m2 ->
+  match_mem R w' m1'_ m2'_ ->
+  Mem.unchanged_on (loc_init_args sz sp2) m2 m2' ->
+  Mem.unchanged_on (not_init_args sz sp2) m2'_ m2' ->
+  exists m1',
+    match_mem R w' m1' m2' /\
+    Mem.unchanged_on (loc_init_args sz sp1) m1 m1' /\
+    Mem.unchanged_on (not_init_args sz sp1) m1'_ m1'.
+Proof.
+  (** To achieve this, we will need to define a new [Mem.mix]
+    operation of the memory model, corresponding injection and
+    extension preservation properties, and add similar conditions to
+    the definition of CKLRs. *)
+Admitted.
+
+Instance make_locset_cklr R:
+  Monotonic make_locset
+    (|= (- ==> Val.inject @@ [mi R]) ++> match_mem R ++> Val.inject @@ [mi R] ++>
+        (- ==> Val.inject @@ [mi R])).
+Proof.
+  intros w rs1 rs2 Hrs m1 m2 Hm sp1 sp2 Hsp l.
+  unfold make_locset, load_stack. rauto.
+Qed.
+
+(** With this, we can state and prove the commutation property. *)
+
+Instance commut_locset_mach R:
+  Commutes cc_locset_mach (cc_locset R) (cc_mach R).
+Proof.
+  intros [[_ w] wR] se1 se2 q1 q2 [[ ] Hse] (qi & Hq1i & Hqi2).
+  destruct Hqi2. inv Hq1i. set (ls2 := make_locset rs2 m2 sp2).
+  transport H11.
+  eexists (se2, (sg, wR'), lmw sg rs2 m2 _). cbn. repeat apply conj; auto.
+  - eapply match_stbls_acc; eauto.
+  - exists (lq vf2 sg ls2 x). split.
+    + constructor; auto; try rauto.
+      * intros l Hl. unfold ls2. rewrite <- HwR'. repeat rstep; auto.
+    + constructor; auto.
+      * destruct H4; congruence.
+  - intros r1 r2 (ri & (wR'' & HwR'' & Hr1i) & Hri2).
+    destruct Hr1i. inv Hri2. rename rs' into rs2'.
+    set (rs1' r := result_regs sg (make_locset rs1 m1 sp1) ls1' (Locations.R r)).
+    edestruct (result_mem R (size_arguments sg) sp1 sp2 wR m1 m2 wR'' m1' m2')
+      as (m1'' & Hm'' & ? & ?); eauto.
+    exists (mr rs1' m1''). split.
+    + constructor; auto.
+      * intros r Hr. unfold rs1'. cbn. destruct in_dec; tauto.
+      * intros r Hr. unfold rs1'. rewrite <- result_regs_agree_callee_save; auto.
+    + exists wR''. split; [rauto | ]. constructor; auto.
+      intro r. unfold rs1', result_regs.
+      destruct in_dec. { rewrite H19; auto. }
+      destruct is_callee_save eqn:Hr; auto.
+      rewrite H20 by auto. cbn. generalize (H5 r).
+      repeat rstep. change (wR ~> wR''). etransitivity; eauto.
+Qed.
+
+(** ** Matching [cc_stacking] *)
+
+(** Next, we show that [cc_stacking] can be reduced to simulation
+  conventions involving [cc_locset_mach]. *)
+
+(** *** Incoming calls *)
+
+Lemma cc_lm_stacking:
+  ccref (cc_locset_mach @ cc_mach inj) (cc_stacking inj).
+Proof.
+  intros [[_ wlm] w] se1 se2 q1 q2 [[ ] Hse] (qi & Hq1i & Hqi2). cbn in *.
+  destruct Hqi2. inv Hq1i.
+  exists (stkw inj w sg (make_locset rs1 m1 sp1) sp2 m2).
+  split; [ | split].
+  - cbn. auto.
+  - constructor; auto.
+    + cbn -[Z.add Z.mul]. repeat apply conj.
+      * apply Mem.unchanged_on_refl.
+      * intros. subst. split.
+        -- destruct H11.
+           ++ apply zero_size_arguments_tailcall_possible in H7.
+              rewrite H7. red. intros. xomega.
+           ++ inversion H2. subst.
+              eapply transport in H7 as (m2_ & Hm2_ & Hm_).
+              2: {
+                change ?x with (id x) in H7. repeat rstep.
+                eapply offset_sarg_ptrrange_inject; eauto.
+                eapply Mem.free_range_perm; eauto.
+                rewrite (offset_sarg_expand (size_arguments sg)).
+                xomega.
+              }
+              eapply Mem.free_range_perm; eauto.
+        -- intros ofs Hofs. destruct H11.
+           ++ apply zero_size_arguments_tailcall_possible in H7.
+              rewrite H7 in Hofs. xomega.
+           ++ inv H2. eapply offset_fits_inject; eauto.
+              eapply Mem.free_range_perm; eauto.
+      * intros ofs ty REG. destruct H11.
+        -- apply tailcall_possible_reg in REG; auto. contradiction.
+        -- edestruct H10 as [v Hv]; eauto. rewrite Hv.
+           transport Hv. rewrite H11. eauto.
+    + destruct H11 as [ | sb1 sofs1 m1 m1_ ]; auto.
+      assert (Mem.extends m1_ m1) by eauto using Mem.free_left_extends, Mem.extends_refl.
+      destruct H6; cbn in *. erewrite <- Mem.mext_next by eauto. constructor.
+      eapply Mem.extends_inject_compose; eauto.
+    + destruct 1. intros b1 delta Hb1 Hp.
+      eapply Mem.perm_free_2; eauto.
+      admit. admit. (* things about injection overlap -- should be okay *)
+    + admit. (* type of sp *)
+    + destruct H4; cbn in *; congruence.
+  - intros r1 r2 Hr. inv Hr.
+    edestruct (result_mem inj (size_arguments sg) sp1 sp2 w m1 m2 w' m1' m2' m2')
+      as (m1'' & ? & ? & ?); eauto using Mem.unchanged_on_refl.
+    set (rs1' r := if is_callee_save r then rs1 r else
+                   if in_dec mreg_eq r (regs_of_rpair (loc_result sg)) then ls1' (R r) else
+                   Vundef).
+    exists (mr rs1' m1''). split.
+    + constructor; auto.
+      * subst rs1'. intros r REG. cbn.
+        destruct in_dec; try contradiction.
+        replace (is_callee_save r) with false; auto.
+        pose proof (loc_result_caller_save sg) as Hr.
+        destruct loc_result; cbn in *; intuition congruence.
+      * subst rs1'. intros r REG. cbn.
+        rewrite REG. congruence.
+    + exists w'; split; auto.
+      constructor; auto.
+      * intros r. subst rs1'. cbn.
+        destruct is_callee_save eqn:CSR; eauto.
+        destruct in_dec; eauto.
+Admitted.
+
+(** *** Outgoing calls *)
+
+Import Separation.
+
+Lemma inject_incr_separated_inv f f' m1 m2 b1 b2 delta:
+  inject_incr f f' ->
+  inject_separated f f' m1 m2 ->
+  f' b1 = Some (b2, delta) ->
+  (Mem.valid_block m1 b1 \/ Mem.valid_block m2 b2) ->
+  f b1 = Some (b2, delta).
+Proof.
+  intros INCR ISEP Hb VALID.
+  destruct (f b1) as [[xb2 xdelta] | ] eqn:Hb1.
+  - apply INCR in Hb1. congruence.
+  - eelim ISEP; eauto. tauto.
+Qed.
+
+Lemma unchanged_on_combine P Q m m' :
+  Mem.unchanged_on P m m' ->
+  Mem.unchanged_on (fun b ofs => Q b ofs /\ ~ P b ofs) m m' ->
+  Mem.unchanged_on Q m m'.
+Proof.
+  clear. intros [ ] [ ].
+  split; intros; eauto; destruct (classic (P b ofs)); eauto.
+Qed.
+
+Lemma cc_stacking_lm:
+  ccref (cc_stacking injp) (cc_locset injp @ cc_locset_mach).
+Proof.
+  intros w se1 se2 q1 q2 Hse Hq. destruct Hq. cbn -[Z.add Z.mul] in * |- .
+  destruct H2 as (UNCH & PERM & ARGS).
+  set (ls2 := make_locset rs2 m2 sp2).
+  (* we'll deal with making sure sp has thee right form later *)
+  assert (exists sb2 sofs2, sp2 = Vptr sb2 sofs2) as (sb2 & sofs2 & Hsp2) by admit.
+  edestruct PERM as [PRNG FITS]; eauto.
+  edestruct (Mem.range_perm_free m2) as (m2_ & Hm2_); eauto.
+  destruct H3; inv Hse; cbn -[Z.add Z.mul] in * |- .
+  eassert (Hm_ : _). {
+    eapply Mem.free_right_inject; eauto.
+    intros. eapply H4; eauto.
+    + constructor; eauto.
+    + replace (ofs + delta - delta) with ofs by xomega.
+    eapply Mem.perm_max, Mem.perm_implies; eauto. constructor.
+  }
+  exists (se2, (sg, injpw _ _ _ Hm_), lmw sg rs2 m2 (Vptr sb2 sofs2)). repeat apply conj.
+  - constructor; cbn; auto. constructor; auto. 
+    erewrite Mem.nextblock_free; eauto.
+  - exists (lq vf2 sg ls2 m2_). split.
+    + constructor; eauto.
+      * intros r Hr. destruct Hr; cbn -[Z.add Z.mul]; eauto.
+        edestruct ARGS as (v2 & Hv2 & Hv); eauto.
+        rewrite Hv2. cbn. auto.
+      * constructor.
+    + econstructor; eauto.
+      * constructor; eauto.
+        -- admit. (* size arguments *)
+        -- intros ofs ty REG. edestruct ARGS as (v2 & Hv2 & Hv); eauto.
+  - intros r1 r2 (ri & (w' & Hw' & Hr1i) & Hri2). cbn -[Z.add Z.mul] in *.
+    inv Hw'. inv Hr1i. inv H3. inv Hri2. cbn -[Z.add Z.mul] in *.
+    rename m1'0 into m1'. rename m2'0 into m2'_. rename m' into m2'.
+    assert (Hm'' : Mem.inject f' m1' m2'). {
+      change (m_pred (minjection f' m1') m2').
+      eapply m_invar; cbn; eauto.
+      eapply Mem.unchanged_on_implies; eauto.
+      intros b2 ofs2 (b1 & delta & Hb & Hp) Hb2 Harg. inv Harg.
+      eapply inject_incr_separated_inv in Hb;
+        eauto using Mem.valid_block_free_1, Mem.perm_valid_block.
+      eapply H4; eauto.
+      * constructor; eauto.
+      * eapply H9; eauto.
+        eapply Mem.valid_block_inject_1; eauto.
+    }
+    exists (injpw f' m1' m2' Hm''); cbn.
+    + constructor; eauto.
+      * intros b ofs p Hb Hp.
+        destruct (classic (loc_init_args (size_arguments sg) (Vptr sb2 sofs2) b ofs)).
+        -- eapply Mem.perm_unchanged_on_2; eauto.
+        -- eapply Mem.perm_free_3; eauto. eapply Mem.valid_block_free_1 in Hb; eauto.
+           eapply H10; eauto. eapply Mem.valid_block_unchanged_on in Hb; eauto.
+           eapply Mem.perm_unchanged_on_2; eauto.
+      * eapply unchanged_on_combine; eauto.
+        apply Mem.unchanged_on_trans with m2_.
+        { eapply Mem.free_unchanged_on; eauto.
+          intros i Hi [Hoor Hlia]. apply Hlia. constructor. eauto. }
+        apply Mem.unchanged_on_trans with m2'_.
+        { eapply Mem.unchanged_on_implies; eauto.
+          tauto. }
+        { eapply Mem.unchanged_on_implies; eauto.
+          intros b ofs [_ ?] _. red. auto. }
+      * red. unfold Mem.valid_block. erewrite <- (Mem.nextblock_free m2); eauto.
+    + intros r REG. rewrite H22; eauto.
+    + intros r REG. rewrite H23; eauto.
+    + constructor.
+    + auto.
+    + intros b2 ofs2 Hofs2 b1 delta Hb Hp.
+      admit.
+(*
+      cut (loc_out_of_reach f m1 b2 ofs2).
+      * intros Hofs2' b1 delta Hb Hp.
+        eapply (Mem.perm_inject f m1' m2'_) in Hp; eauto.
+        replace (ofs2 - delta + delta) with ofs2 in Hp by xomega.
+
+        eapply (Mem.perm_inject f' m1' m2'_) in Hp; eauto.
+        replace (ofs2 - delta + delta) with ofs2 in Hp by xomega.
+ b1 delta Hb Hp. inv Hofs2.
+      erewrite <- Mem.unchanged_on_perm in Hp; eauto.
+      eapply Mem.perm_free_2; eauto.
+      * clear b1 delta Hb Hp. intros b1 delta Hb Hp.
+*)
+Admitted.
+
+(** *** Typing of [cc_locset_mach] source state *)
+
+(** This only works for [Archi.ptr64 = true], in which case there are
+  no actual constraints on register typing. But we need to rely on
+  this for now because of the way callee-save register preservation is
+  formulated in the stacking proof: there is only a guarantee that the
+  original query's source-level register still inject into the reply's
+  target-level registers, but there is no guarantee that the
+  target-level registers are actually unchanged. This means that on
+  incoming calls, [cc_locset_mach] must occur first, before the [inj]
+  component, if we are to satisfy the associated preservation property.
+  But this means that the [lessdef_loc] component which we must insert
+  after [wt_loc] for commutation purposes cannot be absorbed into
+  [inj], and for similar reasons it cannot be folded into
+  [cc_stacking] either.
+
+  So we work around it using the following properties. *)
+
+Lemma type_of_chunk_of_type ty:
+  type_of_chunk (chunk_of_type ty) = ty.
+Proof.
+  destruct ty; cbn; auto.
+Qed.
+
+Lemma always_has_mreg_type v r:
+  Val.has_type v (mreg_type r).
+Proof.
+  unfold mreg_type. change Archi.ptr64 with true.
+  destruct v, r; cbn; auto.
+Qed.
+
+Lemma wt_loc_out_of_thin_air:
+  cceqv (wt_loc @ cc_locset_mach) cc_locset_mach.
+Proof.
+  split.
+  - intros [[xse [xxse sg]] w] se1 se2 q1 q2 [[Hsei] Hse] (_ & [Hq1] & Hq).
+    inv Hsei. inv Hq1. exists w; repeat apply conj; auto.
+    intros r1 r2 Hr. destruct Hr; cbn in *.
+    eexists. split; constructor; auto. constructor.
+    intros r Hr. apply always_has_mreg_type.
+  - intros w se _ q1 q2 [ ] Hq. destruct Hq.
+    exists (se, (se, sg), lmw sg rs m sp). cbn. repeat apply conj; auto.
+    + constructor. auto.
+    + eexists. split; constructor; auto. constructor.
+      intros l Hl. destruct Hl.
+      * apply always_has_mreg_type.
+      * cbn -[Z.add Z.mul]. rewrite <- (type_of_chunk_of_type ty) at 2.
+        destruct sp; cbn -[Z.add Z.mul]; auto.
+        destruct Mem.load eqn:Hl; cbn; auto.
+        eapply Mem.load_type. eauto.
+    + intros r1 r2 (_ & [Hr1] & Hr). auto.
+Qed.
+
+Instance wt_loc_qprop R:
+  PropagatesQueryInvariant (cc_locset R) wt_loc.
+Proof.
+  constructor. cbn.
+  intros [sg wR] [? xsg] se1 se2 q1 q2 Hse Hxse Hq Hq2. subst. inv Hq. inv Hq2.
+  exists (se1, sg). split; auto. constructor.
+  intros. eapply val_has_type_inject; eauto. red. eauto.
+Qed.
+
+Instance wt_loc_rprop R:
+  PropagatesReplyInvariant (cc_locset R) wt_loc.
+Proof.
+  constructor. cbn.
+  intros [se ?] [sg wR] [? ?] se1 se2 q1 q2 r1 r2 Hse ? ? Hq Hq1 Hq2 (wR' & HwR' & Hr) Hr2.
+  subst. inv Hq. inv Hq1. inv Hq2. inv Hr. inv Hr2. constructor.
+  intros. eapply val_has_type_inject; eauto. red. eauto.
+Qed.
+
+
